Changes from J. Villadsen: - removed redundant update_identity - removed requirement "x is different from y" in c6 - proof improvements to frame_property, sound_modusponens, soundness - other minor refactorings

FOL_Monk/FOL_Monk.thy
@@ -1,7 +1,7 @@
 (*
   FOL-Monk - First-Order Logic According to Monk
 
-  Author: John Bruntse Larsen, Andreas HalkjÃ¦r From & JÃ¸rgen Villadsen
+  Author: John Bruntse Larsen, Andreas Halkjær From & Jørgen Villadsen
 *)
 
 theory FOL_Monk imports Main
@@ -28,17 +28,17 @@ primrec vars :: "arity \<Rightarrow> var list"
 
 primrec semantics :: "(var \<Rightarrow> 'a) \<Rightarrow> (string \<Rightarrow> 'a list \<Rightarrow> bool) \<Rightarrow> form \<Rightarrow> bool"
   where
-    "semantics e g (Eq x y) = (e x = e y)" |
     "semantics e g (Pre i n) = g i (map e (vars n))" |
-    "semantics e g (Neg f) = (\<not> semantics e g f)" |
+    "semantics e g (Eq x y) = (e x = e y)" |
+    "semantics e g (Neg p) = (\<not> semantics e g p)" |
     "semantics e g (Imp p q) = (semantics e g p \<longrightarrow> semantics e g q)" |
-    "semantics e g (Uni x p) = (\<forall>t. (semantics (e(x := t)) g p))"
+    "semantics e g (Uni x p) = (\<forall>t. semantics (e(x := t)) g p)"
 
 section \<open>Definition of Rules and Axioms\<close>
 
 primrec not_occurs_in :: "var \<Rightarrow> form \<Rightarrow> bool"
   where
-    "not_occurs_in x (Pre _ arity) = (x \<ge> arity)" |
+    "not_occurs_in x (Pre _ n) = (x \<ge> n)" |
     "not_occurs_in x (Eq y z) = (x \<noteq> y \<and> x \<noteq> z)" |
     "not_occurs_in x (Neg p) = not_occurs_in x p" |
     "not_occurs_in x (Imp p q) = (not_occurs_in x p \<and> not_occurs_in x q)" |
@@ -87,7 +87,7 @@ definition c5_3 :: "var \<Rightarrow> var \<Rightarrow> form \<Rightarrow> thm"
 
 definition c6 :: "var \<Rightarrow> var \<Rightarrow> thm"
   where
-    "c6 x y \<equiv> if x \<noteq> y then Thm (Neg (Uni x (Neg (Eq x y)))) else fail_thm"
+    "c6 x y \<equiv> Thm (Neg (Uni x (Neg (Eq x y))))"
 
 definition c7 :: "var \<Rightarrow> var \<Rightarrow> var \<Rightarrow> thm"
   where
@@ -127,28 +127,21 @@ inductive OK :: "form \<Rightarrow> bool" ("\<turnstile> _" 0)
     "\<turnstile> concl (c8 _ _ _)"
 
 proposition "\<turnstile> Truth"
-  by (metis OK.simps c8_def thm.sel)
+   using case_c6 unfolding c6_def by simp
 
 section \<open>Soundness of Proof System\<close>
-
-lemma update_identity: "e x = e y \<Longrightarrow> semantics e g p \<Longrightarrow> semantics (e(x := e y)) g p"
-  by (simp add: fun_upd_idem)
 
 lemma vars_bound: "x \<ge> n \<Longrightarrow> map e (vars n) = map (e(x := t)) (vars n)"
   by (induct n) simp_all
 
 lemma frame_property: "not_occurs_in x p \<Longrightarrow> semantics e g p = semantics (e(x := t)) g p"
 proof (induct p arbitrary: e)
-  case (Pre i n)
+  case (Pre _ n)
   then have "x \<ge> n"
     by simp
   then show ?case
-    using vars_bound by (metis semantics.simps(2))
-next
-  case (Uni y p)
-  then show ?case
-    by (metis fun_upd_twist not_occurs_in.simps(5) semantics.simps(5))
-qed simp_all
+    using vars_bound by (metis semantics.simps(1))
+qed (simp_all add: fun_upd_twist)
 
 lemma commute_uni: "semantics e g (Uni x (Uni y p)) \<Longrightarrow> semantics e g (Uni y (Uni x p))"
   by (metis fun_upd_twist semantics.simps(5))
@@ -176,23 +169,23 @@ qed
 lemma sound_modusponens:
   "semantics e g (concl f) \<Longrightarrow> semantics e g (concl f') \<Longrightarrow>
   semantics e g (concl (modusponens f f'))"
-  by (cases "concl f") (simp_all add: modusponens_def)
+  unfolding modusponens_def by (cases "concl f") simp_all
 
 theorem soundness: "\<turnstile> p \<Longrightarrow> semantics e g p"
 proof (induct p arbitrary: e rule: OK.induct)
-  case (case_modusponens f f')
+  case case_modusponens
   then show ?case
     using sound_modusponens by fast
 next
-  case (case_c5_1 x p)
+  case case_c5_1
   then show ?case
     unfolding c5_1_def using frame_property by fastforce
 next
-  case (case_c5_3 x y p)
+  case case_c5_3
   then show ?case
     unfolding c5_3_def using commute_uni by fastforce
 next
-  case (case_c8 x y p)
+  case case_c8
   then show ?case
     unfolding c8_def using sound_c8 by simp blast
 qed (simp_all add: gen_def c1_def c2_def c3_def c4_def c5_2_def c6_def c7_def)
